src/absyn/print.fs
@@ -54,9 +54,9 @@ let rec typ_to_string x =
       | None -> strBvd btv.v
       | Some x -> x|> typ_to_string)
   | Typ_const v -> Util.format1 "%s" (sli v.v)
-  | Typ_fun(Some x, t1, t2, imp) -> Util.format "%s%s%s %s %s"  [strBvd x; (if imp then "@" else ":"); (t1 |> typ_to_string); (arrow_of_comp_typ t2); (t2|> comp_typ_to_string)]
-  | Typ_fun(None, t1, t2, _) -> Util.format "%s %s %s"  [(t1 |> typ_to_string); (arrow_of_comp_typ t2); (t2|> comp_typ_to_string)]
-  | Typ_univ(a, k, t) ->       Util.format4 "%s:%s %s %s" (strBvd a) (k |> kind_to_string) (arrow_of_comp_typ t) (t|> comp_typ_to_string)
+  | Typ_fun(Some x, t1, t2, imp) -> Util.format "%s%s%s -> %s"  [strBvd x; (if imp then "@" else ":"); (t1 |> typ_to_string); (t2|> comp_typ_to_string)]
+  | Typ_fun(None, t1, t2, _) -> Util.format "%s -> %s"  [(t1 |> typ_to_string); (t2|> comp_typ_to_string)]
+  | Typ_univ(a, k, t) ->       Util.format3 "%s:%s -> %s" (strBvd a) (k |> kind_to_string) (t|> comp_typ_to_string)
   | Typ_refine(x, t, f) ->     Util.format3 "%s:%s{%s}" (strBvd x) (t|> typ_to_string) (f|> typ_to_string)
   | Typ_app(t1, t2, imp) ->    Util.format3 "(%s %s%s)" (t1|> typ_to_string) (if imp then "#" else "") (t2|> typ_to_string)
   | Typ_dep(t, v, imp) ->      Util.format3 "(%s %s%s)" (t|> typ_to_string) (if imp then "#" else "") (v|> exp_to_string)
@@ -70,14 +70,13 @@ let rec typ_to_string x =
       | Fixed t -> t|> typ_to_string
       | Uvar _ when !Options.print_real_names ->  Util.format2 "'U%s : %s"  (Util.string_of_int (Unionfind.uvar_id uv)) (kind_to_string k)
       | Uvar _ ->               Util.format1 "'U%s"  (Util.string_of_int (Unionfind.uvar_id uv)))
-
-and arrow_of_comp_typ c = match c with 
-  | Pure _ -> "=>"
-  | _ -> "->"
   
-and comp_typ_to_string c = match c with 
-  | Pure t -> typ_to_string t
-  | Computation t -> typ_to_string t
+and comp_typ_to_string c = 
+  let t, args = Util.flatten_typ_apps c in
+  match t.t, args with
+  | Typ_const l, [Inl r] when (lid_equals l.v Const.tot_effect_lid && Util.is_function_typ r) -> typ_to_string r
+  | Typ_const l, [Inl r] when (lid_equals l.v Const.ml_effect_lid && not (Util.is_function_typ r)) -> typ_to_string r
+  | _ -> typ_to_string c
 
 and exp_to_string x = match compress_exp x with 
   | Exp_meta(Meta_datainst(e,_)) -> exp_to_string e 
