src/tc/pretype.fs
@@ -73,20 +73,31 @@ and tc_typ' env (t:typ) : typ' * knd =
   | Typ_const i -> 
     let k = Env.lookup_typ_lid env i.v in 
     t.t,k
-    
-  | Typ_fun(xopt, t1, Pure t2, imp) -> 
+     
+  | Typ_fun(xopt, t1, t2, imp) -> 
     let t1' = tc_typ_check env t1 Kind_type in
     let env' = match xopt with 
       | None -> env
       | Some x -> Env.push_local_binding env (Env.Binding_var(x, t1')) in
-    let t2' = tc_typ_check env' t2 Kind_type in
-    Typ_fun(xopt, t1', Pure t2', imp), Kind_type
+    let t2', k2 = tc_typ env' t2 in
+    let cod = match Util.compress_kind k2 with 
+      | Kind_effect -> t2'
+      | Kind_type -> 
+        if Util.is_function_typ t2'
+        then Util.total_comp t2' (* by default, curried functions are Pure *)
+        else Util.ml_comp t2'    (* Otherwise, give them the ML effect *)
+      | kk -> raise (Error(Tc.Errors.expected_typ_of_kind Kind_effect t2' kk, Util.range_of_typ t2 (Tc.Env.get_range env))) in
+    Typ_fun(xopt, t1', cod, imp), Kind_type
 
-  | Typ_univ(a, k1, Pure t1) -> 
+  | Typ_univ(a, k1, t1) -> 
     let k1' = tc_kind env k1 in 
     let env' = Env.push_local_binding env (Env.Binding_typ(a, k1')) in
-    let t1' = tc_typ_check env' t1 Kind_type in 
-    Typ_univ(a, k1', Pure t1'), Kind_type
+    let t1', k = tc_typ env' t1 in 
+    let cod = match k with 
+      | Kind_effect -> t1'  (* Should polymorphic functions be subject to a purity restriction to support a type-erasure semantics. *)
+      | Kind_type -> Util.total_comp t1' 
+      | _ -> raise (Error(Tc.Errors.expected_typ_of_kind Kind_effect t1' k, Util.range_of_typ t1 (Tc.Env.get_range env))) in
+    Typ_univ(a, k1', cod), Kind_type 
 
   | Typ_refine(x, t1, t2) -> 
     let t1' = tc_typ_check env t1 Kind_type in
@@ -170,12 +181,7 @@ and tc_typ_check env t k : typ =
   Tc.Util.keq env (Some t') k' k;
   t'       
 
-and tc_exp env e : exp * typ = match e with
-  | Exp_meta(Meta_info(e, _, p)) -> 
-    let env = Tc.Env.set_range env p in
-    let e, t = tc_exp env e in
-    Exp_meta(Meta_info(e, t, p)), t
-   
+and tc_value env e : exp * typ = match e with
   | Exp_bvar x -> 
     let t = Env.lookup_bvar env x in
     let e, t = Tc.Util.maybe_instantiate env e t in
@@ -198,15 +204,15 @@ and tc_exp env e : exp * typ = match e with
       let rec aux norm env t = 
         let t = compress_typ t in 
         match t.t with
-        | Typ_fun(xopt, targ, Pure tres, implicit) -> 
-            let tres = match xopt with 
-              | None -> tres
-              | Some y -> Util.subst_typ [Inr(y, Util.bvd_to_exp x targ)] tres in
-            Some targ, Some tres, env, (fun x -> x)
-        | Typ_univ(a, k, Pure t) -> 
+        | Typ_fun(xopt, targ, cod, implicit) -> 
+            let cod = match xopt with 
+              | None -> cod
+              | Some y -> Util.subst_typ [Inr(y, Util.bvd_to_exp x targ)] cod in
+            Some targ, Some cod, env, (fun x -> x)
+        | Typ_univ(a, k, t) -> 
             let env = Tc.Env.push_local_binding env (Env.Binding_typ(a, k)) in 
-            let targ, tres, env, gen = aux norm env t in
-            targ, tres, env, (fun x -> Exp_tabs(a, k, gen x))
+            let targ, cod, env, gen = aux norm env t in
+            targ, cod, env, (fun x -> Exp_tabs(a, k, gen x))
         | Typ_uvar _ ->
           aux norm env (fst <| Tc.Util.destruct_function_typ env t None false)
         | _ when not norm ->
@@ -217,7 +223,6 @@ and tc_exp env e : exp * typ = match e with
         | Some t -> 
           let targ, tres, env, gen = aux false env t in
           targ, tres, env, (fun (x,_) -> gen x, t) in
-
     let targ, tres, env, gen = destruct_expected_typ env in 
     let tx, k1 = tc_typ env t1 in
     let _ = match targ with 
@@ -232,7 +237,7 @@ and tc_exp env e : exp * typ = match e with
     let dom = match xvars |> Util.find_opt (fun (y:bvvar) -> bvd_eq x y.v) with
       | None -> None
       | Some _ -> Some x in 
-    let t = withkind Kind_type <| Typ_fun(dom, tx, Pure tres, false) in
+    let t = withkind Kind_type <| Typ_fun(dom, tx, tres, false) in
     let e' = Exp_abs(x, tx, e1') in 
     gen (e', t)
    
@@ -244,7 +249,7 @@ and tc_exp env e : exp * typ = match e with
         let rec aux norm t = 
           let t = compress_typ t in 
           match t.t with 
-            | Typ_univ(b, karg, Pure tres) -> 
+            | Typ_univ(b, karg, tres) -> 
               Tc.Util.keq env None karg k1';
               let tres = Util.subst_typ [Inl(b, Util.bvd_to_typ a karg)] tres in
               karg, Env.set_expected_typ env tres
@@ -256,10 +261,32 @@ and tc_exp env e : exp * typ = match e with
         k1', env in
     let env' = instantiate_both env' in
     let e1', tres = tc_exp (Env.push_local_binding env' (Env.Binding_typ(a, karg))) e1 in 
-    let t = withkind Kind_type <| Typ_univ(a, karg, Pure tres) in
+    let t = withkind Kind_type <| Typ_univ(a, karg, tres) in
     Exp_tabs(a, karg, e1'), t
 
-  | Exp_meta(Meta_desugared(e, Data_app)) -> 
+  | _ -> failwith "impossible"
+
+and tc_exp env e : exp * typ = match e with
+  | Exp_meta(Meta_info(e, _, p)) -> 
+    let env = Tc.Env.set_range env p in
+    let e, t = tc_exp env e in
+    Exp_meta(Meta_info(e, t, p)), t
+
+  | Exp_bvar _  
+  | Exp_fvar _ 
+  | Exp_constant _ 
+  | Exp_abs _ 
+  | Exp_tabs _ -> 
+    let env = match Tc.Env.expected_typ env with 
+      | Some t -> 
+        (match t.k with 
+          | Kind_effect -> Tc.Env.set_expected_typ env (Util.result_typ t)
+          | _ -> env)
+      | _ -> env in
+    let v, t = tc_value env e in
+    v, Util.total_comp t
+
+  | Exp_meta(Meta_desugared(e, Data_app)) -> (* constructor types already have an (Tot) effect annotation on their co-domain *)
     let env = instantiate_both env in
     let env1, topt = Env.clear_expected_typ env in 
     let d, args = Util.uncurry_app e in 
@@ -268,7 +295,7 @@ and tc_exp env e : exp * typ = match e with
     let e = Util.mk_curried_app d args in
     let e, t = tc_exp env1 e in
     check_expected_typ env (Exp_meta(Meta_desugared(e, Data_app))) t
-    
+
   | Exp_meta(Meta_desugared(e, tag)) -> 
     let e, t = tc_exp env e in
     Exp_meta(Meta_desugared(e, tag)), t
@@ -313,7 +340,7 @@ and tc_exp env e : exp * typ = match e with
     let env1, _ = Env.clear_expected_typ env in
     let e1', t1 = tc_exp ({env1 with Tc.Env.instantiate_vargs=not imp}) e1 in
     let xopt, env2, tres, e1' = match Tc.Util.destruct_function_typ env t1 (Some e1') imp with 
-      | {t=Typ_fun(xopt, targ, Pure tres, _)}, Some e1' -> 
+      | {t=Typ_fun(xopt, targ, tres, _)}, Some e1' -> 
         let env2 = Env.set_expected_typ env targ in
         xopt, env2, tres, e1'
       | _ -> failwith "impossible" in 
@@ -328,7 +355,7 @@ and tc_exp env e : exp * typ = match e with
     let e1', t_e1 = tc_exp ({env1 with Env.instantiate_targs=false}) e1 in 
     let t1', k = tc_typ env1 t1 in 
     begin match Tc.Util.destruct_poly_typ env1 t_e1 e1' t1 with
-      | {t=Typ_univ(a, k', Pure tres)}, e1' ->
+      | {t=Typ_univ(a, k', tres)}, e1' ->
           Tc.Util.keq env1 (Some t1) k k';
           let t = Util.subst_typ [Inl(a, t1')] tres in
           check_expected_typ env (Exp_tapp(e1', t1')) t  
@@ -580,10 +607,13 @@ and tc_decl env se = match se with
     | Sig_datacon(lid, t, tname, r) -> 
       let env = Tc.Env.set_range env r in
       let t = tc_typ_check env t Kind_type in 
-      let args, result_t = Util.collect_formals t in
+      let args, eff = Util.collect_formals t in
+      let result_t = match destruct eff Const.tot_effect_lid with 
+        | Some [Inl t] -> t
+        | _ -> failwith (Util.format1 "Impossible: constructors must have a total effect; got %s\n" (Print.typ_to_string t)) in
       let constructed_t, _ = Util.flatten_typ_apps result_t in (* TODO: check that the tps in tname are the same as here *)
-      let _ = match constructed_t with
-        | {t=Typ_const fv} when lid_equals fv.v tname -> ()
+      let _ = match destruct constructed_t tname with 
+        | Some _ -> ()
         | _ -> raise (Error (Tc.Errors.constructor_builds_the_wrong_type (Util.fvar lid (range_of_lid lid)) constructed_t (Util.ftv tname), range_of_lid lid)) in
       let se = Sig_datacon(lid, t, tname, r) in 
       let env = Tc.Env.push_sigelt env se in 
